A nice logic :-)

proofs/itrees/it_sems_core.v
@@ -90,19 +90,8 @@ error; MF: mutual flat; DE: double error; DF double flat) *)
 (**** ERROR SEMANTICS *******************************************)
 Section Errors.
 
-(* type of errors (this might becom richer) *)
-  (* Variant ErrType : Type := Err : ErrType. *)
 (* error events *)
-
-
 Definition ErrEvent : Type -> Type := exceptE error_data.
-
-(*
-sem_I : prog -> estate -> instr -> itree syscall_Event (state_error + estate)
-sem_i : prog -> estate -> instr_r -> itree syscall_Event (state_error + estate)
-sem_c : prog -> estate -> cmd -> itree syscall_Event (state_error + estate)
-sem_fun : prog -> mem -> syscall -> funname -> values -> itree syscall_Event (state_error + (mem * syscall * values))
-*)
 
 (* failT (itree E) R = itree E (option R) *)
 Definition handle_Err {E} : ErrEvent ~> execT (itree E) :=
@@ -143,7 +132,6 @@ End Errors.
 Section WSW.
 Context
   {asm_op: Type}
-  {asmop: asmOp asm_op}
   {wsw: WithSubWord}
   {dc: DirectCall}
   {syscall_state : Type}
@@ -151,133 +139,143 @@ Context
   {spp : SemPexprParams}
   {sip : SemInstrParams asm_op syscall_state}
   {pT : progT}
-  {scP : semCallParams}
-  (pr : prog)
-  (ev : extra_val_t).
+  {scP : semCallParams}.
 
 Definition mk_error_data (s:estate) (e:error)  := (e, tt).
 
 Definition mk_errtype := fun s => mk_error_data s ErrType.
 
-Definition iget_fundef {E} `{ErrEvent -< E}
-  (fn: funname) (s:estate) : itree E fundef :=
-  ioget (mk_errtype s) (get_fundef (p_funcs pr) fn).
+Section CORE.
 
-Definition iresult  {E} `{ErrEvent -< E} {T} (s:estate) (F : exec T)  : itree E T :=
+Context {E} `{ErrEvent -< E} (p : prog) (ev : extra_val_t).
+
+Definition iget_fundef (funcs: fun_decls) (fn: funname) (s:estate) : itree E fundef :=
+  ioget (mk_errtype s) (get_fundef funcs fn).
+
+Definition iresult {T} (s:estate) (F : exec T)  : itree E T :=
   err_result (mk_error_data s) F.
 
-Definition iwrite_var {E} `{ErrEvent -< E}
-   (wdb : bool) (x : var_i) (v : value) (s : estate) : itree E estate :=
+Definition iwrite_var (wdb : bool) (x : var_i) (v : value) (s : estate) : itree E estate :=
   iresult s (write_var wdb x v s).
 
-Definition iwrite_lval {E} `{ErrEvent -< E}
-   (wdb : bool) (gd : glob_decls) (x : lval) (v : value) (s : estate) : itree E estate :=
+Definition iwrite_lval (wdb : bool) (gd : glob_decls) (x : lval) (v : value) (s : estate) : itree E estate :=
   iresult s (write_lval wdb gd x v s).
 
-Definition iwrite_lvals {E} `{ErrEvent -< E}
-   (wdb : bool) (gd : glob_decls) (s : estate) (xs : lvals) (vs : values) : itree E estate :=
+Definition iwrite_lvals (wdb : bool) (gd : glob_decls) (s : estate) (xs : lvals) (vs : values) : itree E estate :=
   iresult s (write_lvals wdb gd s xs vs).
 
-Definition isem_pexpr {E} `{ErrEvent -< E}
-   (wdb : bool) (gd : glob_decls) (s : estate) (e: pexpr) : itree E value :=
+Definition isem_pexpr (wdb : bool) (gd : glob_decls) (s : estate) (e: pexpr) : itree E value :=
   iresult s (sem_pexpr wdb gd s e).
 
-Definition isem_pexprs {E} `{ErrEvent -< E}
-   (wdb : bool) (gd : glob_decls) (s : estate) (es: pexprs) : itree E values :=
+Definition isem_pexprs (wdb : bool) (gd : glob_decls) (s : estate) (es: pexprs) : itree E values :=
   iresult s (sem_pexprs wdb gd s es).
 
-Definition eval_assgn
-  (x: lval) (tg: assgn_tag) (ty: stype) (e: pexpr)
-  (st1: estate) : exec estate :=
-   (Let v := sem_pexpr true (p_globs pr) st1 e in
+Definition sem_assgn  (x : lval) (tg : assgn_tag) (ty : stype) (e : pexpr) (s : estate) : exec estate :=
+   (Let v := sem_pexpr true (p_globs p) s e in
     Let v' := truncate_val ty v in
-    write_lval true (p_globs pr) x v' st1).
+    write_lval true (p_globs p) x v' s).
 
-Definition eval_syscall
-   (xs: lvals) (o: syscall_t)
-   (es: pexprs) (s: estate) : exec estate :=
-  Let ves := sem_pexprs true (p_globs pr) s es in
+Definition sem_syscall (xs : lvals) (o : syscall_t) (es : pexprs) (s : estate) : exec estate :=
+  Let ves := sem_pexprs true (p_globs p) s es in
   Let: (scs, m, vs) := exec_syscall s.(escs) s.(emem) o ves in
-  write_lvals true (p_globs pr)
+  write_lvals true (p_globs p)
      (with_scs (with_mem s m) scs) xs vs.
+
+Definition sem_cond (gd : glob_decls) (e : pexpr) (s : estate) : exec bool :=
+  sem_pexpr true gd s e >>r= to_bool.
+
+Definition isem_cond (e : pexpr) (s : estate) : itree E bool :=
+  iresult s (sem_cond (p_globs p) e s).
+
+Definition sem_bound (gd : glob_decls) (lo hi : pexpr) (s : estate) : exec (Z * Z) :=
+  Let vlo := sem_pexpr true gd s lo >>r= to_int in
+  Let vhi := sem_pexpr true gd s hi >>r= to_int in
+  ok (vlo, vhi).
+
+Definition isem_bound (lo hi : pexpr) (s : estate) : itree E (Z * Z) :=
+  iresult s (sem_bound (p_globs p) lo hi s).
 
 (** Auxiliary functions for recursion on list (seq) *)
 
-Fixpoint isem_cmd_body {E} (sem_i: instr -> estate -> itree E estate)
-   (c: cmd) (st: estate) : itree E estate :=
+End CORE.
+
+Section SEM_C.
+
+Context {E} `{ErrEvent -< E}
+        (sem_i: prog -> extra_val_t -> instr -> estate -> itree E estate)
+        (p : prog) (ev : extra_val_t).
+
+Fixpoint isem_cmd_body (c: cmd) (s: estate) : itree E estate :=
   match c with
-  | nil => Ret st
-  | i :: c' => st' <- sem_i i st ;; isem_cmd_body sem_i c' st'
+  | nil => Ret s
+  | i :: c' => s' <- sem_i p ev i s ;; isem_cmd_body c' s'
   end.
 
-Fixpoint isem_for_body {E} `{ErrEvent -< E}
-   (sem_i : instr -> estate -> itree E estate)
-   (i: var_i) (c: cmd)
-   (ls: list Z) (s: estate) : itree E estate :=
+Fixpoint isem_for_body (i : var_i) (c : cmd) (ls : list Z) (s : estate) : itree E estate :=
   match ls with
   | nil => ret s
   | (w :: ws) =>
     s <- iwrite_var true i (Vint w) s;;
-    s <- isem_cmd_body sem_i c s;;
-    isem_for_body sem_i i c ws s
+    s <- isem_cmd_body c s;;
+    isem_for_body i c ws s
   end.
 
 (* Make global definition *)
 Local Notation continue_loop st := (ret (inl st)).
 Local Notation exit_loop st := (ret (inr st)).
 
-Local Notation gd := (p_globs pr).
-
-Definition isem_cond {E} `{ErrEvent -< E} (e:pexpr) (s: estate) : itree E bool :=
-  iresult s (sem_pexpr true gd s e >>r= to_bool).
-
-Definition isem_bound {E} `{ErrEvent -< E} (e:pexpr) (s: estate) :
-   itree E Z :=
-  iresult s (sem_pexpr true gd s e >>r= to_int).
-
-Definition isem_while_loop {E} `{ErrEvent -< E}
-   (sem_i : instr -> estate -> itree E estate)
-   (c1 : cmd) (e:pexpr) (c2: cmd) (s1 : estate) : itree E (estate + estate) :=
-   s2 <- isem_cmd_body sem_i c1 s1 ;;
-   b <- isem_cond e s2 ;;
-   if b then s3 <- isem_cmd_body sem_i c2 s2 ;; continue_loop s3
+Definition isem_while_loop (c1 : cmd) (e : pexpr) (c2 : cmd) (s1 : estate) : itree E (estate + estate) :=
+   s2 <- isem_cmd_body c1 s1 ;;
+   b <- isem_cond p e s2 ;;
+   if b then s3 <- isem_cmd_body c2 s2 ;; continue_loop s3
    else exit_loop s2.
 
-Definition isem_while_body {E} `{ErrEvent -< E}
-   (sem_i : instr -> estate -> itree E estate)
-   (c1 : cmd) (e:pexpr) (c2: cmd) (s1 : estate) : itree E estate :=
-  ITree.iter (isem_while_loop sem_i c1 e c2) s1.
+Definition isem_while_body (c1 : cmd) (e:pexpr) (c2: cmd) (s1 : estate) : itree E estate :=
+  ITree.iter (isem_while_loop c1 e c2) s1.
+
+End SEM_C.
 
 Record fstate := { fscs : syscall_state_t; fmem : mem; fvals : values }.
 
-Fixpoint isem_i_body {E} `{ErrEvent -< E}
-   (sem_call : funname -> fstate -> itree E fstate)
-   (i: instr) (s1: estate) : itree E estate :=
-  let sem_i := isem_i_body sem_call in
-  let sem_cmd := isem_cmd_body sem_i in
+Section SEM_I.
+
+Context {E} `{ErrEvent -< E} (sem_fun : prog -> extra_val_t -> funname -> fstate -> itree E fstate).
+
+Fixpoint isem_i_body (p : prog) (ev : extra_val_t) (i : instr) (s1 : estate) : itree E estate :=
   let: (MkI _ i) := i in
   match i with
-  | Cassgn x tg ty e => iresult s1 (eval_assgn x tg ty e s1)
-  | Copn xs tg o es => iresult s1 (sem_sopn gd o s1 xs es)
-  | Csyscall xs o es => iresult s1 (eval_syscall xs o es s1)
+  | Cassgn x tg ty e => iresult s1 (sem_assgn p x tg ty e s1)
+  | Copn xs tg o es => iresult s1 (sem_sopn (p_globs p) o s1 xs es)
+  | Csyscall xs o es => iresult s1 (sem_syscall p xs o es s1)
 
   | Cif e c1 c2 =>
-    b <- isem_cond e s1;;
-    sem_cmd (if b then c1 else c2) s1
+    b <- isem_cond p e s1;;
+    isem_cmd_body isem_i_body p ev (if b then c1 else c2) s1
 
   | Cwhile a c1 e c2 =>
-    isem_while_body sem_i c1 e c2 s1
+    isem_while_body isem_i_body p ev c1 e c2 s1
 
   | Cfor i (d, lo, hi) c =>
-    vlo <- isem_bound lo s1 ;;
-    vhi <- isem_bound hi s1 ;;
-    isem_for_body sem_i i c (wrange d vlo vhi) s1
+    bounds <- isem_bound p lo hi s1 ;;
+    isem_for_body isem_i_body p ev i c (wrange d bounds.1 bounds.2) s1
 
   | Ccall xs fn args =>
-    vargs <- isem_pexprs  (~~direct_call) gd s1 args;;
-    r <- sem_call fn {| fscs := escs s1; fmem:= emem s1; fvals := vargs |} ;;
-    iwrite_lvals (~~direct_call) gd (with_scs (with_mem s1 r.(fmem)) r.(fscs)) xs r.(fvals)
+    vargs <- isem_pexprs  (~~direct_call) (p_globs p) s1 args;;
+    r <- sem_fun p ev fn {| fscs := escs s1; fmem:= emem s1; fvals := vargs |} ;;
+    iwrite_lvals (~~direct_call) (p_globs p) (with_scs (with_mem s1 r.(fmem)) r.(fscs)) xs r.(fvals)
   end.
+
+Definition isem_cmd_ := isem_cmd_body isem_i_body.
+
+Lemma isem_cmd_cat p ev c c' s :
+  isem_cmd_ p ev (c ++ c') s ≈ (s' <- isem_cmd_ p ev c s;; isem_cmd_ p ev c' s').
+Proof.
+  rewrite /isem_cmd_; elim: c s => [ | i c hc] /= s.
+  + rewrite bind_ret_l; reflexivity.
+  rewrite bind_bind; setoid_rewrite hc; reflexivity.
+Qed.
+
+End SEM_I.
 
 (**********************************************************************)
 (** error-aware interpreter with mutual recursion *)
@@ -285,66 +283,74 @@ Fixpoint isem_i_body {E} `{ErrEvent -< E}
 Variant recCall : Type -> Type :=
  | RecCall (f:funname) (fs:fstate) : recCall fstate.
 
-(* Make global definition *)
-
-Definition rec_call  {E} `{ErrEvent -< E} (f:funname) (fs:fstate) : itree (recCall +' E) fstate :=
- trigger_inl1 (RecCall f fs).
-
-Definition isem_i_rec {E} `{ErrEvent -< E} (i : instr) (s1: estate) : itree (recCall +' E) estate :=
-  isem_i_body rec_call i s1.
-
 Definition estate0 (fs : fstate) :=
   Estate fs.(fscs) fs.(fmem) Vm.init.
 
-Definition initialize_call (fd:fundef) (fs:fstate) : exec estate :=
+Definition initialize_funcall (p : prog) (ev : extra_val_t) (fd : fundef) (fs : fstate) : exec estate :=
   let sinit := estate0 fs in
   Let vargs' := mapM2 ErrType dc_truncate_val fd.(f_tyin) fs.(fvals) in
-  Let s0 := init_state fd.(f_extra) (p_extra pr) ev sinit in
+  Let s0 := init_state fd.(f_extra) (p_extra p) ev sinit in
   write_vars (~~direct_call) fd.(f_params) vargs' s0.
 
-Definition finalize_call (fd : fundef) (s:estate) :=
+Definition finalize_funcall (fd : fundef) (s:estate) :=
   Let vres := get_var_is (~~ direct_call) s.(evm) fd.(f_res) in
   Let vres' := mapM2 ErrType dc_truncate_val fd.(f_tyout) vres in
   let scs := s.(escs) in
   let m := finalize fd.(f_extra) s.(emem) in
   ok {| fscs := scs; fmem := m; fvals := vres' |}.
 
-Definition isem_call_body {E} `{ErrEvent -< E}
-   (rec_call : funname -> fstate -> itree E fstate)
-   (fn : funname) (fs:fstate) : itree E fstate :=
+Definition isem_fun_body {E} `{ErrEvent -< E}
+   (rec_call : prog -> extra_val_t -> funname -> fstate -> itree E fstate)
+   (p : prog) (ev : extra_val_t)
+   (fn : funname) (fs : fstate) : itree E fstate :=
   (* FIXME: this is durty : sinit*)
   let sinit := estate0 fs in
-  fd <- iget_fundef fn sinit;;
-  s1 <- iresult sinit (initialize_call fd fs);;
-  s2 <- isem_cmd_body (isem_i_body rec_call) fd.(f_body) s1;;
-  iresult s2 (finalize_call fd s2).
+  fd <- iget_fundef (p_funcs p) fn sinit;;
+  s1 <- iresult sinit (initialize_funcall p ev fd fs);;
+  s2 <- isem_cmd_ rec_call p ev fd.(f_body) s1;;
+  iresult s2 (finalize_funcall fd s2).
 
-Definition isem_call_rec {E} `{ErrEvent -< E}
-   (fn : funname) (fs:fstate) : itree (recCall +' E) fstate :=
-  isem_call_body rec_call fn fs.
+Section SEM_F.
 
-Definition interp_recCall {E} `{ErrEvent -< E} : recCall ~> itree (recCall +' E) :=
+Context {E} `{ErrEvent -< E}.
+
+Definition rec_call (p : prog) (ev : extra_val_t) (f : funname) (fs : fstate) : itree (recCall +' E) fstate :=
+ trigger_inl1 (RecCall f fs).
+
+Definition isem_i_rec (p : prog) (ev : extra_val_t) (i : instr) (s1 : estate) : itree (recCall +' E) estate :=
+  isem_i_body rec_call p ev i s1.
+
+Definition isem_cmd_rec (p : prog) (ev : extra_val_t) (c : cmd) (s1 : estate) : itree (recCall +' E) estate :=
+  isem_cmd_ rec_call p ev c s1.
+
+Definition isem_fun_rec (p : prog) (ev : extra_val_t)
+   (fn : funname) (fs : fstate) : itree (recCall +' E) fstate :=
+  isem_fun_body rec_call p ev fn fs.
+
+Definition interp_recCall (p : prog) (ev : extra_val_t) : recCall ~> itree (recCall +' E) :=
  fun T (rc : recCall T) =>
    match rc with
-   | RecCall fn fs => isem_call_rec fn fs
+   | RecCall fn fs => isem_fun_rec p ev fn fs
    end.
 
-Definition isem_call {E} `{ErrEvent -< E} (fn : funname) (fs : fstate) : itree E fstate :=
-  mrec interp_recCall (RecCall fn fs).
+Definition isem_fun (p : prog) (ev : extra_val_t) (fn : funname) (fs : fstate) : itree E fstate :=
+  mrec (interp_recCall p ev) (RecCall fn fs).
 
-Definition isem_i {E} `{ErrEvent -< E} (i : instr) (s : estate) : itree E estate :=
-  isem_i_body isem_call i s.
+Definition isem_i (p : prog) (ev : extra_val_t) (i : instr) (s : estate) : itree E estate :=
+  isem_i_body isem_fun p ev i s.
 
-Definition isem_cmd {E} `{ErrEvent -< E} (c : cmd) (s : estate) : itree E estate :=
-  isem_cmd_body isem_i c s.
+Definition isem_cmd (p : prog) (ev : extra_val_t) (c : cmd) (s : estate) : itree E estate :=
+  isem_cmd_ isem_fun p ev c s.
 
-Definition sem_call (fn : funname) (fs : fstate) : execT (itree void1) (fstate) :=
-  interp_Err (isem_call fn fs).
+End SEM_F.
+
+Definition sem_fun (p : prog) (ev : extra_val_t) (fn : funname) (fs : fstate) : execT (itree void1) (fstate) :=
+  interp_Err (isem_fun p ev fn fs).
 
 (* Core lemmas about the definition *)
 
-Lemma interp_ioget {E : Type -> Type} `{ErrEvent -< E} Err T (o : option T) :
-  eutt (E:=E) eq (interp (mrecursive interp_recCall) (ioget Err o)) (ioget Err o).
+Lemma interp_ioget {E : Type -> Type} `{ErrEvent -< E} (p : prog) (ev : extra_val_t) Err T (o : option T) :
+  eutt (E:=E) eq (interp (mrecursive (interp_recCall p ev)) (ioget Err o)) (ioget Err o).
 Proof.
   case o => /=.
   + move=> ?; rewrite interp_ret; reflexivity.
@@ -352,8 +358,8 @@ Proof.
   by apply eqit_Vis => -[].
 Qed.
 
-Lemma interp_iresult {E : Type -> Type} `{ErrEvent -< E} s T (r : exec T) :
-  eutt (E:=E) eq (interp (mrecursive interp_recCall) (iresult s r)) (iresult s r).
+Lemma interp_iresult {E : Type -> Type} `{ErrEvent -< E} (p : prog) (ev : extra_val_t) s T (r : exec T) :
+  eutt (E:=E) eq (interp (mrecursive (interp_recCall p ev)) (iresult s r)) (iresult s r).
 Proof.
   case r => /=.
   + move=> ?; rewrite interp_ret; reflexivity.
@@ -361,21 +367,22 @@ Proof.
   by apply eqit_Vis => -[].
 Qed.
 
-Lemma interp_isem_cmd {E} `{ErrEvent -< E} c s :
-  eutt (E:=E) eq (interp (mrecursive interp_recCall) (isem_cmd_body (isem_i_body rec_call) c s))
-    (isem_cmd_body (isem_i_body isem_call) c s).
+Lemma interp_isem_cmd {E} `{ErrEvent -< E} (p : prog) (ev : extra_val_t) c s :
+  eutt (E:=E) eq (interp (mrecursive (interp_recCall p ev)) (isem_cmd_body isem_i_rec p ev c s))
+         (isem_cmd_body (isem_i_body isem_fun) p ev c s).
 Proof.
-  apply: (cmd_rect
+  apply:
+   (cmd_rect
     (Pr := fun ir => forall ii s,
-       eutt (E:=E) eq (interp (mrecursive interp_recCall) (isem_i_rec (MkI ii ir) s))
-                      (isem_i (MkI ii ir) s))
+       eutt (E:=E) eq (interp (mrecursive (interp_recCall p ev)) (isem_i_rec p ev (MkI ii ir) s))
+                      (isem_i p ev (MkI ii ir) s))
     (Pi := fun i => forall s,
-       eutt (E:=E) eq (interp (mrecursive interp_recCall) (isem_i_rec i s))
-                      (isem_i i s))
+       eutt (E:=E) eq (interp (mrecursive (interp_recCall p ev)) (isem_i_rec p ev i s))
+                      (isem_i p ev i s))
     (Pc := fun c => forall s,
-       eutt (E:=E) eq (interp (mrecursive interp_recCall) (isem_cmd_body isem_i_rec c s))
-                      (isem_cmd c s))) c s => //=.
-  + move=> s; rewrite interp_ret; reflexivity.
+       eutt (E:=E) eq (interp (mrecursive (interp_recCall p ev)) (isem_cmd_body isem_i_rec p ev c s))
+                      (isem_cmd p ev c s))) => // {c s}.
+  + move=> s /=; rewrite interp_ret; reflexivity.
   + move=> i c hi hc s; rewrite interp_bind;apply eqit_bind; first by apply hi.
     by move=> s'; apply hc.
   + by move=> >; apply interp_iresult.
@@ -387,9 +394,7 @@ Proof.
     by move=> []; [apply hc1 | apply hc2].
   + move=> v dir lo hi c hc ii s; rewrite /isem_i /isem_i_rec /=.
     rewrite interp_bind; apply eqit_bind; first by apply interp_iresult.
-    move=> vlo.
-    rewrite interp_bind; apply eqit_bind; first by apply interp_iresult.
-    move=> vhi; elim: wrange s => {vlo vhi ii} //=.
+    move=> bounds; elim: wrange s => {bounds ii} //=.
     + move=> >; rewrite interp_ret; reflexivity.
     move=> j js hrec s.
     rewrite interp_bind; apply eqit_bind; first by apply interp_iresult.
@@ -411,12 +416,12 @@ Proof.
   rewrite interp_mrecursive; reflexivity.
 Qed.
 
-Lemma isem_call_unfold {E} `{ErrEvent -< E} (fn : funname) (fs : fstate) :
-  isem_call (E:=E) fn fs ≈ isem_call_body isem_call fn fs.
+Lemma isem_call_unfold {E} `{ErrEvent -< E} (p : prog) (ev : extra_val_t) (fn : funname) (fs : fstate) :
+  isem_fun (E:=E) p ev fn fs ≈ isem_fun_body isem_fun p ev fn fs.
 Proof.
-  rewrite {1}/isem_call.
+  rewrite {1}/isem_fun.
   rewrite mrec_as_interp.
-  rewrite {2}/interp_recCall /isem_call_rec /isem_call_body.
+  rewrite {2}/interp_recCall /isem_fun_rec /isem_fun_body.
   rewrite interp_bind; apply eqit_bind.
   + by apply interp_ioget.
   move=> fd; rewrite interp_bind; apply eqit_bind.
@@ -427,5 +432,3 @@ Proof.
 Qed.
 
 End WSW.
-
-
