proofs/itrees/it_sems_core_proofs.v
@@ -67,11 +67,9 @@ Import MonadNotation.
 Local Open Scope monad_scope.
 Local Open Scope option_scope.
 
-(*
 Set Implicit Arguments.
 Unset Strict Implicit.
 Unset Printing Implicit Defensive.
-*)
 
 (* PROBLEM with sections *)
 
@@ -98,10 +96,10 @@ Definition rutt_err {E1 E2: Type -> Type}
   {HasErr1: ErrEvent -< E1} {wE1 : with_Error E1}
   {HasErr2: ErrEvent -< E2} {wE2 : with_Error E2}
   {O1 O2 : Type}
-  (pre_event : prerel E1 E2)
-  (post_event: postrel E1 E2)
+  (RpreInv : prerel E1 E2)
+  (RpostInv: postrel E1 E2)
   (post      : O1 -> O2 -> Prop) :=
-  @rutt E1 E2 O1 O2 ErrorCutoff NoCutoff pre_event post_event post.
+  @rutt E1 E2 O1 O2 ErrorCutoff NoCutoff RpreInv RpostInv post.
 
 Instance with_Error_suml {E: Type -> Type} {HasErr: ErrEvent -< E} {wE : with_Error E} (T:Type -> Type) :
   with_Error (T +' E).
@@ -132,68 +130,234 @@ Proof.
   admit. (* this is ht modulo extentional equality *)
 Admitted.
 
+Lemma rutt_err_weaken {E1 E2: Type -> Type}
+  {HasErr1: ErrEvent -< E1} {wE1 : with_Error E1}
+  {HasErr2: ErrEvent -< E2} {wE2 : with_Error E2}
+  {O1 O2 : Type}
+  (RpreInv : prerel E1 E2)
+  (RpostInv: postrel E1 E2)
+  (post post' : O1 -> O2 -> Prop) t1 t2 :
+  (forall o1 o2, post o1 o2 -> post' o1 o2) ->
+  rutt_err RpreInv RpostInv post t1 t2 ->
+  rutt_err RpreInv RpostInv post' t1 t2.
+Admitted.
 
+Definition rel (I1 I2 : Type) := I1 -> I2 -> Prop.
 
+Definition relIO (I1 I2 O1 O2 : Type) := I1 -> I2 -> O1 -> O2 -> Prop.
 
+Section REQUIV.
 
+Context {E:Set}.
 
+Definition fresult T1 T2 := T1 -> result E T2.
 
-(*
-Existing Instance HasErr.
- *)
-(*
+Definition requiv_io {I1 I2 O1 O2}
+   (P : rel I1 I2) (F1 : fresult I1 O1) (F2 : fresult I2 O2) (Q : relIO I1 I2 O1 O2) :=
+  forall i1 i2 o1, P i1 i2 -> F1 i1 = ok o1 -> exists2 o2, F2 i2 = ok o2 & Q i1 i2 o1 o2.
 
+Definition requiv {I1 I2 O1 O2}
+   (P : rel I1 I2) (F1 : fresult I1 O1) (F2 : fresult I2 O2) (Q : rel O1 O2) :=
+  requiv_io P F1 F2 (fun _ _ => Q).
 
+Lemma requiv_io_weaken {I1 I2 O1 O2} (P P' : rel I1 I2) (Q Q': relIO I1 I2 O1 O2) F1 F2 :
+  (forall i1 i2, P' i1 i2 -> P i1 i2) ->
+  (forall i1 i2 o1 o2, P' i1 i2 -> Q i1 i2 o1 o2 -> Q' i1 i2 o1 o2) ->
+  requiv_io P F1 F2 Q ->
+  requiv_io P' F1 F2 Q'.
+Proof.
+  move=> hP'P hQQ' h i1 i2 o1 hP' hF1.
+  have [o2 -> hQ]:= h _ _ _ (hP'P _ _ hP') hF1; eauto.
+Qed.
 
-Section CUTOFF.
+Lemma requiv_weaken {I1 I2 O1 O2} (P P' : rel I1 I2) (Q Q': rel O1 O2) F1 F2 :
+  (forall i1 i2, P' i1 i2 -> P i1 i2) ->
+  (forall o1 o2, Q o1 o2 -> Q' o1 o2) ->
+  requiv P F1 F2 Q ->
+  requiv P' F1 F2 Q'.
+Proof. move=> hP'P hQQ'; apply requiv_io_weaken => //; auto. Qed.
 
+Lemma requiv_io_ok {I1 I2} (P:rel I1 I2) (Q: relIO I1 I2 I1 I2):
+  (forall i1 i2, P i1 i2 -> Q i1 i2 i1 i2) ->
+  requiv_io P (@Ok _ _) (@Ok _ _) Q.
+Proof. by move=> hPQ i1 i2 o1 hQ [<-]; exists i2 => //; apply hPQ. Qed.
 
+Lemma requiv_ok {I1 I2} (Q:rel I1 I2) : requiv Q (@Ok _ _) (@Ok _ _) Q.
+Proof. by apply requiv_io_ok. Qed.
 
-Context (E: Type -> Type).
-Context (HasErr: ErrEvent -< E).
+Lemma requiv_io_err {I1 I2 O1 O2} (P:rel I1 I2) (Q: relIO I1 I2 O1 O2) (Err : E) F :
+  requiv_io P (fun i1 => Error Err) F Q.
+Proof. by move=> ?. Qed.
 
-Context (E0: Type -> Type).
-Context (FI: FIso (E0 +' ErrEvent) E).
+Lemma requiv_err {I1 I2 O1 O2} (P:rel I1 I2) (Q: rel O1 O2) (Err : E) F :
+  requiv P (fun i1 => Error Err) F Q.
+Proof. apply requiv_io_err. Qed.
 
-Definition ErrorCutoff X (m : E X) :=
-  match mfun2 _ m with
-  | inl1 _ => true
-  | inr1 x => false
-  end.
+Lemma requiv_io_bind {I1 I2 T1 T2 O1 O2}
+  (R : relIO I1 I2 T1 T2)
+  (P : rel I1 I2)
+  (Q : relIO I1 I2 O1 O2) F1 F1' F2 F2' :
+  requiv_io P F1 F2 R ->
+  (forall i1 i2, P i1 i2 -> requiv (R i1 i2) F1' F2' (Q i1 i2)) ->
+  requiv_io P (fun i => F1 i >>r= F1') (fun i => F2 i >>r= F2') Q.
+Proof.
+  move=> h h' i1 i2 o1 hP; t_xrbindP => t1 /(h _ _ _ hP) [t2 -> /= hR].
+  by apply: h'.
+Qed.
 
-Definition NoCutoff : forall X, E X -> bool :=
-  fun X m => true.
+Lemma requiv_bind {I1 I2 T1 T2 O1 O2}
+  (R : rel T1 T2)
+  (P : rel I1 I2)
+  (Q : rel O1 O2) F1 F1' F2 F2' :
+  requiv P F1 F2 R ->
+  requiv R F1' F2' Q ->
+  requiv P (fun i => F1 i >>r= F1') (fun i => F2 i >>r= F2') Q.
+Proof. by move=> h h'; apply requiv_io_bind with (R:= fun _ _ => R). Qed.
 
-End CUTOFF.
+Lemma requiv_mapM {I1 I2 O1 O2} (P : rel I1 I2) (Q : rel O1 O2) F1 F2 :
+  requiv P F1 F2 Q ->
+  requiv (List.Forall2 P) (mapM F1) (mapM F2) (List.Forall2 Q).
+Proof.
+  move=> heqv s1; elim: s1 => [ | i1 is1 hrec] [ | i2 is2] os /List_Forall2_inv //=.
+  + by move=> _ [<-]; eauto.
+  move=> [hP halli]; t_xrbindP => o1 ho1 os1 hos1 <-.
+  have [o2 -> /= hQ] := heqv _ _ _ hP ho1.
+  have [os2 -> /= hallo] := hrec _ _ halli hos1; eauto.
+Qed.
 
-*)
+Lemma requiv_fold2 {A1 B1 A2 B2 R1 R2} (Err : E)
+  (I: rel R1 R2) (PA : rel A1 A2) (PB : rel B1 B2)
+  (F1 : A1 -> B1 -> R1 -> result E R1) (F2 : A2 -> B2 -> R2 -> result E R2)
+  (la1 : seq A1) (la2 : seq A2) (lb1 : seq B1) (lb2 : seq B2) :
+  Forall2 PA la1 la2 ->
+  Forall2 PB lb1 lb2 ->
+  (forall a1 a2 b1 b2, PA a1 a2 -> PB b1 b2 -> requiv I (F1 a1 b1) (F2 a2 b2) I) ->
+  requiv I (fold2 Err F1 la1 lb1) (fold2 Err F2 la2 lb2) I.
+Proof.
+  move=> halla hallb hF.
+  elim: halla lb1 lb2 hallb => {la1 la2}.
+  + by move=> _ _ [] => //=; apply requiv_ok.
+  move=> a1 a2 la1 la2 hPA halla hrec _ _ [] => //= b1 b2 lb1 lb2 hPB hallb.
+  apply requiv_bind with I; auto.
+Qed.
+
+End REQUIV.
+
+Class relEvent (E : Type -> Type) :=
+  { HasErr1  :: ErrEvent -< E
+  ; wE      :: with_Error E
+  ; RPreInv  :: prerel E E
+  ; RPostInv :: postrel E E }.
+
+Section IEQUIV.
+
+Context {E: Type -> Type} {rE : relEvent E}.
+
+Definition fitree E (I O : Type) := I -> itree E O.
+
+Definition iequiv_io {I1 I2 O1 O2}
+   (P : rel I1 I2) (F1 : fitree E I1 O1) (F2 : fitree E I2 O2) (Q : relIO I1 I2 O1 O2) :=
+  forall i1 i2, P i1 i2 -> rutt_err RPreInv RPostInv (Q i1 i2) (F1 i1) (F2 i2).
+
+Definition iequiv {I1 I2 O1 O2}
+   (P : rel I1 I2) (F1 : fitree E I1 O1) (F2 : fitree E I2 O2) (Q : rel O1 O2) :=
+   iequiv_io P F1 F2 (fun i1 i2 => Q).
+
+Lemma iequiv_io_weaken {I1 I2 O1 O2} (P P' : rel I1 I2) (Q Q': relIO I1 I2 O1 O2) F1 F2 :
+  (forall i1 i2, P' i1 i2 -> P i1 i2) ->
+  (forall i1 i2 o1 o2, P' i1 i2 -> Q i1 i2 o1 o2 -> Q' i1 i2 o1 o2) ->
+  iequiv_io P F1 F2 Q ->
+  iequiv_io P' F1 F2 Q'.
+Proof.
+  move=> hP'P hQQ' heqv i1 i2 hP'.
+  apply rutt_err_weaken with (Q i1 i2).
+  + by move=> >; apply hQQ'.
+  by apply/heqv/hP'P.
+Qed.
+
+Lemma iequiv_weaken {I1 I2 O1 O2} (P P' : rel I1 I2) (Q Q': rel O1 O2) F1 F2 :
+  (forall i1 i2, P' i1 i2 -> P i1 i2) ->
+  (forall o1 o2, Q o1 o2 -> Q' o1 o2) ->
+  iequiv P F1 F2 Q ->
+  iequiv P' F1 F2 Q'.
+Proof. move=> hP hQ; apply iequiv_io_weaken => // > _; apply hQ. Qed.
+
+Lemma iequiv_io_ret {I1 I2} (P: rel I1 I2) (Q : relIO I1 I2 I1 I2) :
+  (forall i1 i2, P i1 i2 -> Q i1 i2 i1 i2) ->
+  iequiv_io P (fun i => Ret i) (fun i => Ret i) Q.
+Proof. by move=> hPQ i1 i2 hP; apply/rutt_Ret/hPQ. Qed.
+
+Lemma iequiv_ret {I1 I2} (Q: rel I1 I2) :
+  iequiv Q (fun i => Ret i) (fun i => Ret i) Q.
+Proof. by apply iequiv_io_ret. Qed.
+
+(* comp_pre P Q o1 o2 <-> exists i1 i2, P i1 i2 /\ Q i1 i2 o1 o2 *)
+Variant comp_pre {I1 I2 O1 O2} (P : rel I1 I2) (Q: relIO I1 I2 O1 O2) (o1 : O1) (o2 : O2) : Prop :=
+  | Comp_io : forall i1 i2, P i1 i2 -> Q i1 i2 o1 o2 -> comp_pre P Q o1 o2.
+
+Definition comp_post {I1 I2 T1 T2 O1 O2}
+   (P : rel I1 I2) (R : relIO I1 I2 T1 T2) (Q : relIO I1 I2 O1 O2)
+   (t1 : T1) (t2 : T2) (o1 : O1) (o2 : O2) :=
+  forall i1 i2, P i1 i2 -> R i1 i2 t1 t2 -> Q i1 i2 o1 o2.
+
+Lemma iequiv_io_bind {I1 I2 T1 T2 O1 O2}
+  (R : relIO I1 I2 T1 T2)
+  (P : rel I1 I2)
+  (Q : relIO I1 I2 O1 O2) F1 F1' F2 F2' :
+  iequiv_io P F1 F2 R ->
+  (forall i1 i2, P i1 i2 -> iequiv (R i1 i2) F1' F2' (Q i1 i2)) ->
+  iequiv_io P (fun i => t <- F1 i;; F1' t) (fun i => t <- F2 i;; F2' t) Q.
+Proof.
+  move=> h h' i1 i2 hP.
+  apply rutt_bind with (R i1 i2); first by apply h.
+  by move=> t1 t2 hR; apply h'.
+Qed.
+
+Lemma iequiv_bind {I1 I2 T1 T2 O1 O2}
+  (R : rel T1 T2)
+  (P : rel I1 I2)
+  (Q : rel O1 O2) F1 F1' F2 F2' :
+  iequiv P F1 F2 R ->
+  iequiv R F1' F2' Q ->
+  iequiv P (fun i => t <- F1 i;; F1' t) (fun i => t <- F2 i;; F2' t) Q.
+Proof. by move=> h h'; apply iequiv_io_bind with (R := fun t1 t2 => R). Qed.
+
+End IEQUIV.
+
+(* Definition of a relational logic over program *)
+
 Section WSW.
+
 Context
-  {asm_op: Type}
-  {asmop: asmOp asm_op}
-  {wsw: WithSubWord}
-  {dc: DirectCall}
   {syscall_state : Type}
   {ep : EstateParams syscall_state}
   {spp : SemPexprParams}
+  {asm_op: Type}
   {sip : SemInstrParams asm_op syscall_state}
-  {pT : progT}
-  {scP : semCallParams}
-  (ev : extra_val_t).
+  {pT1 pT2 : progT}
+  {wsw1 wsw2: WithSubWord}
+  {scP1 : semCallParams (wsw:= wsw1) (pT := pT1)}
+  {scP2 : semCallParams (wsw:= wsw2) (pT := pT2)}
+  {dc1 dc2: DirectCall}.
 
-Section Section.
+Notation prog1 := (prog (pT := pT1)).
+Notation prog2 := (prog (pT := pT2)).
 
-Context {E1 E2: Type -> Type}
-        {HasErr1 : ErrEvent -< E1} {HasErr2 : ErrEvent -< E2}
-        {wE1 : with_Error E1} {wE2 : with_Error E2}
-        (TR_E : forall T1 T2,
-            E1 T1 -> E2 T2 -> Prop)
-        (VR_E : forall T1 T2,
-            E1 T1 -> T1 -> E2 T2 -> T2 -> Prop).
+Notation extra_val_t1 := (@extra_val_t pT1).
+Notation extra_val_t2 := (@extra_val_t pT2).
 
-Lemma rutt_iresult (T1 T2:Type) st1 st2 (x1 : exec T1) (x2 : exec T2) (R : T1 -> T2 -> Prop) :
+Notation estate1 := (estate (wsw:=wsw1) (ep:=ep)).
+Notation estate2 := (estate (wsw:=wsw2) (ep:=ep)).
+
+Notation isem_fun1 := (isem_fun (wsw:=wsw1) (dc:=dc1) (ep:=ep) (spp:=spp) (sip:=sip) (pT:=pT1) (scP:= scP1)).
+Notation isem_fun2 := (isem_fun (wsw:=wsw2) (dc:=dc2) (ep:=ep) (spp:=spp) (sip:=sip) (pT:=pT2) (scP:= scP2)).
+
+Section IRESULT.
+Context {E: Type -> Type} {rE: relEvent E}.
+
+Lemma rutt_iresult (T1 T2:Type) (s1 : estate1) (s2 : estate2) (x1 : exec T1) (x2 : exec T2) (R : T1 -> T2 -> Prop) :
   (forall v1, x1 = ok v1 -> exists2 v2, x2 = ok v2 & R v1 v2) ->
-  rutt_err TR_E VR_E R (iresult st1 x1) (iresult st2 x2).
+  rutt_err RPreInv RPostInv R (iresult s1 x1) (iresult s2 x2).
 Proof.
   case: x1 => [ v1 | e1] hok.
   + have [v2 -> /=] := hok _ erefl.
@@ -202,643 +366,496 @@ Proof.
   by rewrite /ErrorCutoff /= is_error_has.
 Qed.
 
-End Section.
+End IRESULT.
 
-(***************************************************************************)
-(*** APPLICATION ***********************************************************)
-(** we define a language translation and try to prove equivalence of
-function application and commands across the translation under the
-appropriate hypothesis. First we specify the translation. *)
+Class sem_call_2 {E : Type -> Type} {rE: relEvent E} :=
+ { sem_call1 : prog1 -> extra_val_t1 -> funname -> fstate -> itree E fstate
+ ; sem_call2 : prog2 -> extra_val_t2 -> funname -> fstate -> itree E fstate }.
 
-(*** TRANSLATION SPEC *******************************************)
-Section TRANSF.
+#[global]
+Instance sc2_full {E : Type -> Type} {rE: relEvent E} : sem_call_2 | 100 :=
+  {| sem_call1 := isem_fun1
+   ; sem_call2 := isem_fun2 |}.
+
+Section TR_MutualRec.
+
+Context (RPreF : funname -> funname -> fstate -> fstate -> Prop).
+Context (RPostF : funname -> funname -> fstate -> fstate -> fstate -> fstate -> Prop).
+
+Context {E: Type -> Type} {rE:relEvent E}.
+
+Definition RPreD {T1 T2} (d1 : recCall T1)
+                         (d2 : recCall T2) : Prop :=
+  match d1, d2 with
+  | RecCall fn1 fs1, RecCall fn2 fs2 => RPreF fn1 fn2 fs1 fs2
+  end.
+
+Definition RPostD {T1 T2} (d1 : recCall T1) (t1: T1) (d2 : recCall T2) (t2: T2) : Prop :=
+  match d1 in recCall T1_ return T1_ -> T2 -> Prop with
+  | RecCall fn1 fs1 =>
+    match d2 in recCall T2_ return fstate -> T2_ -> Prop with
+    | RecCall fn2 fs2 => RPostF fn1 fn2 fs1 fs2
+    end
+  end t1 t2.
+
+Definition relEvent_recCall : relEvent (recCall +' E).
+econstructor.
++ apply with_Error_suml.
++ exact (sum_prerel (@RPreD) RPreInv).
++ exact (sum_postrel (@RPostD) RPostInv).
+Defined.
+
+Definition sc2_rec : sem_call_2 (rE := relEvent_recCall) :=
+  {| sem_call1 := rec_call (E:=E)
+   ; sem_call2 := rec_call (E:=E) |}.
+
+End TR_MutualRec.
+
+Section EQUIV_CORE.
+
+Context {E : Type -> Type} {rE: relEvent E}.
+
+Lemma iequiv_iresult (P Q : rel estate1 estate2) (F1 : estate1 -> exec estate1) (F2: estate2 -> exec estate2) :
+  requiv P F1 F2 Q ->
+  iequiv P (fun s => iresult s (F1 s)) (fun s => iresult s (F2 s)) Q.
+Proof. by move=> h s1 s2 hP; apply rutt_iresult => s1'; apply: h. Qed.
+
+Context {SC2 : sem_call_2} (p1 : prog1) (p2 : prog2) (ev1: extra_val_t1) (ev2 : extra_val_t2).
+
+Definition relPreF := funname -> funname -> fstate -> fstate -> Prop.
+Definition relPostF := funname -> funname -> fstate -> fstate -> fstate -> fstate -> Prop.
+
+Definition rel_c := rel estate1 estate2.
+
+Definition equiv_f (P : relPreF) (fn1 fn2 : funname) (Q:relPostF) :=
+  iequiv_io (P fn1 fn2) (sem_call1 p1 ev1 fn1) (sem_call2 p2 ev2 fn2) (Q fn1 fn2).
+
+Definition equiv_f_body (P : relPreF) (fn1 fn2 : funname) (Q:relPostF) :=
+  iequiv_io (P fn1 fn2)
+            (isem_fun_body (dc:=dc1) sem_call1 p1 ev1 fn1) (isem_fun_body (dc:=dc2) sem_call2 p2 ev2 fn2)
+            (Q fn1 fn2).
+
+Definition equiv (pre:rel_c) (c1 c2 : cmd) (post : rel_c) :=
+  iequiv pre (isem_cmd_ (dc:=dc1) sem_call1 p1 ev1 c1) (isem_cmd_ (dc:=dc2) sem_call2 p2 ev2 c2) post.
+
+Lemma equiv_weaken P1 P2 Q1 Q2 c1 c2 :
+  (forall s1 s2, P1 s1 s2 -> P2 s1 s2) ->
+  (forall s1 s2, Q2 s1 s2 -> Q1 s1 s2) ->
+  equiv P2 c1 c2 Q2 ->
+  equiv P1 c1 c2 Q1.
+Proof. by apply iequiv_weaken. Qed.
+
+Lemma equiv_cat (R P Q : rel_c) (c1 c1' c2 c2' : cmd) :
+  equiv P c1 c2 R ->
+  equiv R c1' c2' Q ->
+  equiv P (c1 ++ c1') (c2 ++ c2') Q.
+Proof.
+  move=> h h' s1 s2 hP; rewrite !isem_cmd_cat.
+  apply rutt_bind with R; first by apply h.
+  apply h'.
+Qed.
+
+Lemma equiv_nil Q : equiv Q [::] [::] Q.
+Proof. apply iequiv_ret. Qed.
+
+Lemma equiv_cons (R P Q : rel_c) (i1 i2 : instr) (c1 c2 : cmd) :
+  equiv P [::i1] [::i2] R ->
+  equiv R c1 c2 Q ->
+  equiv P (i1 :: c1) (i2 :: c2) Q.
+Proof. rewrite -(cat1s i1 c1) -(cat1s i2 c2); apply equiv_cat. Qed.
+
+Lemma equiv_assgn (Re Rtr: value -> value -> Prop) P Q ii1 x1 tg1 ty1 e1 ii2 x2 tg2 ty2 e2 :
+  requiv P (fun s => sem_pexpr true (p_globs p1) s e1)
+           (fun s => sem_pexpr true (p_globs p2) s e2) Re ->
+  requiv Re (truncate_val ty1) (truncate_val ty2) Rtr ->
+  (forall v1 v2, Rtr v1 v2 ->
+    requiv P (write_lval true (p_globs p1) x1 v1) (write_lval true (p_globs p2) x2 v2) Q) ->
+  equiv P [:: MkI ii1 (Cassgn x1 tg1 ty1 e1)] [:: MkI ii2 (Cassgn x2 tg2 ty2 e2)] Q.
+Proof.
+  move=> he htr hwr; rewrite /equiv /isem_cmd_ /=.
+  apply iequiv_bind with Q; last apply iequiv_ret.
+  apply iequiv_iresult; rewrite /sem_assgn.
+  move=> s1 s2 s1' hP; rewrite /sem_assgn.
+  t_xrbindP => v1 /(he _ _ _ hP) [v2 -> /= hv] v1' /(htr _ _ _ hv) [v2' ->] hv' /=.
+  by apply hwr.
+Qed.
+
+Lemma equiv_opn (Rve Rvo : values -> values -> Prop) P Q ii1 xs1 at1 o1 es1 ii2 xs2 at2 o2 es2 :
+  requiv P (fun s => sem_pexprs true (p_globs p1) s es1)
+           (fun s => sem_pexprs true (p_globs p2) s es2) Rve ->
+  requiv Rve (exec_sopn o1) (exec_sopn o2) Rvo ->
+  (forall vs1 vs2,
+    Rvo vs1 vs2 -> requiv P (fun s1 => write_lvals true (p_globs p1) s1 xs1 vs1)
+                            (fun s2 => write_lvals true (p_globs p2) s2 xs2 vs2) Q) ->
+  equiv P [:: MkI ii1 (Copn xs1 at1 o1 es1)] [:: MkI ii2 (Copn xs2 at2 o2 es2)] Q.
+Proof.
+  move=> he ho hwr; rewrite /equiv /isem_cmd_ /=.
+  apply iequiv_bind with Q; last apply iequiv_ret.
+  apply iequiv_iresult.
+  move=> s1 s2 s1' hP; rewrite /sem_sopn.
+  t_xrbindP => vr1 v1 /(he _ _ _ hP) [v2 -> /= hv]  /(ho _ _ _ hv) [v2' ->] hv' /=.
+  by apply hwr.
+Qed.
+
+Lemma equiv_syscall Rve Rvo P Q ii1 xs1 sc1 es1 ii2 xs2 sc2 es2 :
+  requiv P (fun s => sem_pexprs true (p_globs p1) s es1)
+           (fun s => sem_pexprs true (p_globs p2) s es2) Rve ->
+  (forall ves1 ves2,
+     Rve ves1 ves2 ->
+     requiv P (fun (s:estate1) => exec_syscall (pT:=pT1) (escs s) (emem s) sc1 ves1)
+              (fun (s:estate2) => exec_syscall (pT:=pT2) (escs s) (emem s) sc2 ves2) Rvo) ->
+  (forall scs1 m1 vs1 scs2 m2 vs2,
+    Rvo (scs1, m1, vs1) (scs2, m2, vs2) ->
+    requiv P (fun s => write_lvals true (p_globs p1) (with_scs (with_mem s m1) scs1) xs1 vs1)
+             (fun s => write_lvals true (p_globs p2) (with_scs (with_mem s m2) scs2) xs2 vs2) Q) ->
+  equiv P [:: MkI ii1 (Csyscall xs1 sc1 es1)] [:: MkI ii2 (Csyscall xs2 sc2 es2)] Q.
+Proof.
+  move=> he ho hwr; rewrite /equiv /isem_cmd_ /=.
+  apply iequiv_bind with Q; last apply iequiv_ret.
+  apply iequiv_iresult.
+  move=> s1 s2 s1' hP; rewrite /sem_syscall.
+  t_xrbindP => v1 /(he _ _ _ hP) [v2 -> /= hv] [[scs1 m1] v1'].
+  move=> /(ho _ _ hv _ _ _ hP) [[[scs2 m2] v2'] -> hv'] /= hw.
+  by apply: hwr hP hw.
+Qed.
+
+Lemma equiv_if_full P Q ii1 e1 c1 c1' ii2 e2 c2 c2' :
+  requiv P (sem_cond (p_globs p1) e1) (sem_cond (p_globs p2) e2) eq ->
+  equiv (fun s1 s2 => [/\ P s1 s2, sem_cond (p_globs p1) e1 s1 = ok true & sem_cond (p_globs p2) e2 s2 = ok true])
+        c1 c2 Q ->
+  equiv (fun s1 s2 => [/\ P s1 s2, sem_cond (p_globs p1) e1 s1 = ok false & sem_cond (p_globs p2) e2 s2 = ok false])
+        c1' c2' Q ->
+  equiv P [:: MkI ii1 (Cif e1 c1 c1')] [:: MkI ii2 (Cif e2 c2 c2')] Q.
+Proof.
+  move=> he hc hc' s1 s2 hP; rewrite /isem_cmd_ /=.
+  apply rutt_bind with Q; last by move=> >; apply rutt_Ret.
+  apply rutt_bind with (fun b1 b2 =>
+     [/\ b1 = b2, sem_cond (p_globs p1) e1 s1 = ok b1 & sem_cond (p_globs p2) e2 s2 = ok b2]).
+  + by apply/rutt_iresult => b1 he1; have [b2 he2 heq] := he _ _ _ hP he1; exists b2.
+  by move=> [] _ [<- ??]; [apply hc | apply hc'].
+Qed.
+
+Lemma equiv_if P Q ii1 e1 c1 c1' ii2 e2 c2 c2' :
+  requiv P (sem_cond (p_globs p1) e1) (sem_cond (p_globs p2) e2) eq ->
+  equiv P c1 c2 Q ->
+  equiv P c1' c2' Q ->
+  equiv P [:: MkI ii1 (Cif e1 c1 c1')] [:: MkI ii2 (Cif e2 c2 c2')] Q.
+Proof.
+  move=> hcond hc hc'; apply equiv_if_full => //.
+  + by apply: equiv_weaken hc => // > [].
+  by apply: equiv_weaken hc' => // > [].
+Qed.
+
+Lemma equiv_for P Pi ii1 i1 d lo1 hi1 c1 ii2 i2 lo2 hi2 c2 :
+  requiv P (sem_bound (p_globs p1) lo1 hi1) (sem_bound (p_globs p2) lo2 hi2) eq ->
+  (forall i : Z, requiv P (write_var true i1 (Vint i)) (write_var true i2 (Vint i)) Pi) ->
+  equiv Pi c1 c2 P ->
+  equiv P [:: MkI ii1 (Cfor i1 (d, lo1, hi1) c1)] [:: MkI ii2 (Cfor i2 (d, lo2, hi2) c2)] P.
+Proof.
+  move=> hbound hwi hc s1 s2 hP; rewrite /isem_cmd_ /=.
+  apply rutt_bind with P; last by move=> >; apply rutt_Ret.
+  apply rutt_bind with eq.
+  + by apply rutt_iresult => >; apply hbound.
+  move=> [vlo vhi] _ <- /=; elim: wrange s1 s2 hP=> [|j js hrec] /= s1 s2 hP.
+  + by apply rutt_Ret.
+  apply rutt_bind with Pi.
+  + by apply rutt_iresult => >; apply hwi.
+  move=> r1 r2 hPi; apply rutt_bind with P => //.
+  by apply hc.
+Qed.
+
+Lemma equiv_while_full I I' ii1 al1 e1 c1 c1' ii2 al2 e2 c2 c2' :
+  equiv I c1 c2 I' ->
+  requiv I' (sem_cond (p_globs p1) e1) (sem_cond (p_globs p2) e2) eq ->
+  equiv (fun s1 s2 =>
+    [/\ I' s1 s2, sem_cond (p_globs p1) e1 s1 = ok true & sem_cond (p_globs p2) e2 s2 = ok true]) c1' c2' I ->
+  equiv I [:: MkI ii1 (Cwhile al1 c1 e1 c1')] [:: MkI ii2 (Cwhile al2 c2 e2 c2')]
+     (fun s1 s2 => [/\ I' s1 s2, sem_cond (p_globs p1) e1 s1 = ok false & sem_cond (p_globs p2) e2 s2 = ok false]).
+Proof.
+  move=> hc hcond hc' s1 s2 hI; rewrite /isem_cmd_ /=.
+  set Q := (fun s1 s2 =>
+    [/\ I' s1 s2, sem_cond (p_globs p1) e1 s1 = ok false & sem_cond (p_globs p2) e2 s2 = ok false]).
+  apply rutt_bind with Q; last by move=> >; apply rutt_Ret.
+  rewrite /isem_while_body; apply XRuttFacts.rutt_iter with (RI := I) => //.
+  move=> {}s1 {}s2 {}hI; rewrite /isem_while_loop.
+  apply rutt_bind with I'; first by apply hc.
+  move=> {hI} {}s1 {}s2 hI'.
+  apply rutt_bind with
+    (fun b1 b2 => [/\ b1 = b2, sem_cond (p_globs p1) e1 s1 = ok b1 & sem_cond (p_globs p2) e2 s2 = ok b2]).
+  + by apply/rutt_iresult => b1 he1; have [b2 he2 heq] := hcond _ _ _ hI' he1; exists b2.
+  move=> [] _ [<- he1 he2].
+  + apply rutt_bind with I; first by apply hc'.
+    by move=> r1 r2 hI; apply rutt_Ret; constructor.
+  by apply rutt_Ret; constructor.
+Qed.
+
+Lemma equiv_while I I' ii1 al1 e1 c1 c1' ii2 al2 e2 c2 c2' :
+  equiv I c1 c2 I' ->
+  requiv I' (sem_cond (p_globs p1) e1) (sem_cond (p_globs p2) e2) eq ->
+  equiv I' c1' c2' I ->
+  equiv I [:: MkI ii1 (Cwhile al1 c1 e1 c1')] [:: MkI ii2 (Cwhile al2 c2 e2 c2')] I'.
+Proof.
+  move=> hc hcond hc'.
+  apply equiv_weaken with (P2 := I)
+    (Q2 := fun s1 s2 =>
+      [/\ I' s1 s2, sem_cond (p_globs p1) e1 s1 = ok false & sem_cond (p_globs p2) e2 s2 = ok false]) => //.
+  + by move=> > [].
+  apply equiv_while_full => //.
+  by apply: equiv_weaken hc' => // > [].
+Qed.
+
+Lemma equiv_call (Pf : relPreF) (Qf : relPostF) Rv P Q ii1 xs1 fn1 es1 ii2 xs2 fn2 es2 :
+  requiv P (fun s => sem_pexprs (~~ (@direct_call dc1)) (p_globs p1) s es1)
+           (fun s => sem_pexprs (~~ (@direct_call dc2)) (p_globs p2) s es2) Rv ->
+  (forall s1 s2 vs1 vs2,
+     P s1 s2 -> Rv vs1 vs2 ->
+     Pf fn1 fn2 {| fscs := escs s1; fmem := emem s1; fvals := vs1 |}
+                {| fscs := escs s2; fmem := emem s2; fvals := vs2 |}) ->
+  equiv_f Pf fn1 fn2 Qf ->
+  (forall fs1 fs2 fr1 fr2,
+    Pf fn1 fn2 fs1 fs2 -> Qf fn1 fn2 fs1 fs2 fr1 fr2 ->
+    requiv (* (fun s1 s2 => [/\ escs s1 = fscs fs1, emem s1 = fmem fs1
+                           , escs s2 = fscs fs2, emem s2 = fmem fs2
+                           & P s1 s2]) *)
+           P
+     (fun s => write_lvals (~~ (@direct_call dc1)) (p_globs p1) (with_scs (with_mem s (fmem fr1)) (fscs fr1)) xs1 (fvals fr1))
+     (fun s => write_lvals (~~ (@direct_call dc2)) (p_globs p2) (with_scs (with_mem s (fmem fr2)) (fscs fr2)) xs2 (fvals fr2))
+    Q) ->
+  equiv P [:: MkI ii1 (Ccall xs1 fn1 es1)] [:: MkI ii2 (Ccall xs2 fn2 es2)] Q.
+Proof.
+  move=> hes hPPf hCall hPQf s1 s2 hP; rewrite /isem_cmd_ /=.
+  apply rutt_bind with Q; last by move=> >; apply rutt_Ret.
+  apply rutt_bind with Rv.
+  + by apply rutt_iresult => >; apply: hes.
+  move=> vs1 vs2 hvs.
+  set fs1 := {| fscs := escs s1 |}; set fs2 := {| fscs := escs s2 |}.
+  apply rutt_bind with (Qf fn1 fn2 fs1 fs2).
+  + by apply/hCall/hPPf.
+  move=> fr1 fr2 hr; apply rutt_iresult => >.
+  apply (hPQf fs1 fs2 fr1 fr2) => //.
+  by apply hPPf.
+Qed.
+
+Definition isem_fun_body_hyp (RPreF:relPreF) fn1 fn2 (RPostF:relPostF) :=
+  forall fs1 fs2,
+  RPreF fn1 fn2 fs1 fs2 ->
+  forall fd1, get_fundef (p_funcs p1) fn1 = Some fd1 ->
+  exists2 fd2, get_fundef (p_funcs p2) fn2 = Some fd2 &
+    exists (P Q : rel_c),
+      forall s11, initialize_funcall (dc:=dc1) p1 ev1 fd1 fs1 = ok s11 ->
+      exists s21,
+        [/\ initialize_funcall (dc:=dc2) p2 ev2 fd2 fs2 = ok s21
+          , P s11 s21
+          , equiv P fd1.(f_body) fd2.(f_body) Q
+          & requiv Q (finalize_funcall (dc:=dc1) fd1) (finalize_funcall (dc:=dc2) fd2) (RPostF fn1 fn2 fs1 fs2)].
+
+Lemma equiv_fun_body RPreF fn1 fn2 RPostF :
+  isem_fun_body_hyp RPreF fn1 fn2 RPostF ->
+  equiv_f_body RPreF fn1 fn2 RPostF.
+Proof.
+  move=> hf fs1 fs2 hpre.
+  rewrite /isem_fun_body.
+  have {}hf := hf _ _ hpre.
+  rewrite /iget_fundef.
+  apply rutt_bind with (fun fd1 fd2 => get_fundef (p_funcs p1) fn1 = Some fd1 /\
+                                        get_fundef (p_funcs p2) fn2 = Some fd2).
+  + case heq: get_fundef => [fd1 | ] /=.
+    + by have [fd2 -> _] := hf _ heq; apply rutt_Ret.
+    by apply rutt_CutL; rewrite /ErrorCutoff /= is_error_has.
+  move=> fd1 fd2 [hfd1 hfd2]; have := hf fd1 hfd1.
+  rewrite hfd2 => -[ _ [<- [P] [Q] {}hf]].
+  apply rutt_bind with (fun s1 s2 => initialize_funcall (dc:=dc1) p1 ev1 fd1 fs1 = ok s1 /\
+                                     initialize_funcall (dc:=dc2) p2 ev2 fd2 fs2 = ok s2).
+  + apply rutt_iresult.
+    by move=> s hs; have [s' [?]] := hf _ hs; eauto.
+  move=> s1 s1' [hs1 hs1']; have := hf _ hs1.
+  rewrite hs1' => -[?] [[<-] hP heqv hpost].
+  apply rutt_bind with Q.
+  + by apply heqv.
+  move=> r1 r2 hQ; apply rutt_iresult.
+  by move=> fr1; apply hpost.
+Qed.
+
+End EQUIV_CORE.
+
+Section EQUIV_FUN.
+
+Context {E : Type -> Type} {rE : relEvent E}.
+
+Context (p1 : prog1) (p2 : prog2) (ev1: extra_val_t1) (ev2 : extra_val_t2).
+
+Definition equiv_f_rec RPreF fn1 fn2 RPostF :=
+  equiv_f (rE:=relEvent_recCall RPreF RPostF) (SC2:=sc2_rec RPreF RPostF) p1 p2 ev1 ev2 RPreF fn1 fn2 RPostF.
+
+Definition equiv_rec (RPreF : relPreF) (RPostF : relPostF) P c1 c2 Q :=
+  equiv (rE:=relEvent_recCall RPreF RPostF) (SC2:=sc2_rec RPreF RPostF) p1 p2 ev1 ev2 P c1 c2 Q.
+
+Definition isem_fun_body_hyp_rec (RPreF:relPreF) fn1 fn2 (RPostF:relPostF) :=
+  forall fs1 fs2,
+  RPreF fn1 fn2 fs1 fs2 ->
+  forall fd1, get_fundef (p_funcs p1) fn1 = Some fd1 ->
+  exists2 fd2, get_fundef (p_funcs p2) fn2 = Some fd2 &
+    exists (P Q : rel_c),
+      forall s11, initialize_funcall (dc:=dc1) p1 ev1 fd1 fs1 = ok s11 ->
+      exists s21,
+        [/\ initialize_funcall (dc:=dc2) p2 ev2 fd2 fs2 = ok s21
+          , P s11 s21
+          , equiv_rec RPreF RPostF P fd1.(f_body) fd2.(f_body) Q
+          & requiv Q (finalize_funcall (dc:=dc1) fd1) (finalize_funcall (dc:=dc2) fd2) (RPostF fn1 fn2 fs1 fs2)].
+
+Lemma isem_fun_ind (RPreF : relPreF) (RPostF : relPostF) :
+  ((forall fn1 fn2, equiv_f_rec RPreF fn1 fn2 RPostF) ->
+   (forall fn1 fn2, isem_fun_body_hyp_rec RPreF fn1 fn2 RPostF)) ->
+  forall fn1 fn2,
+  equiv_f (rE:=rE) (SC2:=sc2_full) p1 p2 ev1 ev2 RPreF fn1 fn2 RPostF.
+Proof.
+  have hrec : (forall fn1 fn2, equiv_f_rec RPreF fn1 fn2 RPostF).
+  + move=> fn1' fn2' fs1' fs2' hpre'; apply rutt_trigger => //.
+    + by apply sum_prerel_inl.
+    by rewrite /RPostInv /= => fr1 fr2 h; dependent destruction h.
+  move=> /(_ hrec) hbody fn1 fn2 fs1 fs2 hpre.
+  apply interp_mrec_rutt_err with (RPreInv := @RPreD RPreF) (RPostInv := @RPostD RPostF).
+  + move=> {hpre fn1 fn2 fs1 fs2}.
+    move=> _ _ [fn1 fs1] [fn2 fs2] /= hpre.
+    by apply (equiv_fun_body (hbody fn1 fn2) hpre).
+  by apply (equiv_fun_body (hbody fn1 fn2) hpre).
+Qed.
+
+End EQUIV_FUN.
+
+End WSW.
+
+Section TEST.
+
+Context
+  {syscall_state : Type}
+  {ep : EstateParams syscall_state}
+  {spp : SemPexprParams}
+  {asm_op: Type}
+  {sip : SemInstrParams asm_op syscall_state}
+  {pT : progT}
+  {wsw: WithSubWord}
+  {scP : semCallParams}
+  {dc: DirectCall}.
+
+Context {E : Type -> Type} {rE : relEvent E}.
+
 Context (tr_lval : lval -> lval)
-        (tr_expr : pexpr -> pexpr)
-        (tr_opn : sopn -> sopn)
-        (tr_sysc : syscall_t -> syscall_t).
+        (tr_expr : pexpr -> pexpr).
 
 Local Notation tr_lvals ls := (map tr_lval ls).
 Local Notation tr_exprs es := (map tr_expr es).
 
-Definition Tr_i (Th: instr_r -> instr_r) (i: instr) : instr :=
-  match i with MkI ii ir => MkI ii (Th ir) end.
+Fixpoint tr_i (i : instr) : instr :=
+  let: (MkI ii i) := i in
+  let i' :=
+    match i with
+    | Cassgn x tg ty e => Cassgn (tr_lval x) tg ty (tr_expr e)
+    | Copn xs tg o es =>
+        Copn (tr_lvals xs) tg o (tr_exprs es)
+    | Csyscall xs sc es =>
+        Csyscall (tr_lvals xs) sc (tr_exprs es)
+    | Cif e c1 c2 => Cif (tr_expr e) (map tr_i c1) (map tr_i c2)
+    | Cfor i (d, lo, hi) c => Cfor i (d, tr_expr lo, tr_expr hi) (map tr_i c)
+    | Cwhile a c1 e c2 => Cwhile a (map tr_i c1) (tr_expr e) (map tr_i c2)
+    | Ccall xs fn es => Ccall (tr_lvals xs) fn (tr_exprs es)
+    end in
+  MkI ii i'.
 
-Fixpoint Tr_ir (i : instr_r) : instr_r :=
-  let R := Tr_i Tr_ir in
-  match i with
-  | Cassgn x tg ty e => Cassgn (tr_lval x) tg ty (tr_expr e)
-  | Copn xs tg o es =>
-      Copn (tr_lvals xs) tg (tr_opn o) (tr_exprs es)
-  | Csyscall xs sc es =>
-      Csyscall (tr_lvals xs) (tr_sysc sc) (tr_exprs es)
-  | Cif e c1 c2 => Cif (tr_expr e) (map R c1) (map R c2)
-  | Cfor i rg c => Cfor i rg (map R c)
-  | Cwhile a c1 e c2 => Cwhile a (map R c1) (tr_expr e) (map R c2)
-  | Ccall xs fn es => Ccall (tr_lvals xs) fn (tr_exprs es)
-  end.
+Local Notation tr_c := (map tr_i).
 
-Local Notation Tr_instr := (Tr_i Tr_ir).
-Local Notation Tr_cmd c := (map Tr_instr c).
+Definition tr_fundef (f: fundef) : fundef :=
+  {| f_info := f_info f
+   ; f_tyin := f_tyin f
+   ; f_params := f_params f
+   ; f_body := tr_c (f_body f)
+   ; f_tyout := f_tyout f
+   ; f_res := f_res f
+   ; f_extra := f_extra f |}.
 
-Definition Tr_FunDef (f: fundef) : fundef :=
-  match f with
-  | MkFun i tyin p_xs c tyout r_xs xtr =>
-    MkFun i tyin p_xs (Tr_cmd c) tyout r_xs xtr end.
+Context (p1 : prog) (ev:extra_val_t).
 
-(*********************************************************************)
-(*** PROOFS **********************************************************)
+Let p2 := map_prog tr_fundef p1.
 
-Section TR_tests.
+Definition RPreFeq (fn1 fn2 : funname) (fs1 fs2 : fstate) := fn1 = fn2 /\ fs1 = fs2.
+Definition RPostFeq (fn1 fn2 : funname) (fs1 fs2 fr1 fr2: fstate) := fr1 = fr2.
 
-Context (pr1 : prog).
+Context (tr_exprP : forall wdb gd e,
+   requiv eq (fun s => sem_pexpr wdb gd s e) (fun s => sem_pexpr wdb gd s (tr_expr e)) eq).
 
-Let pr2 := map_prog Tr_FunDef pr1.
+Context (tr_lvalP : forall wdb gd x v,
+   requiv eq (write_lval wdb gd x v) (write_lval wdb gd (tr_lval x) v) eq).
 
-Context (E: Type -> Type)
-        (TR_E : forall T1 T2,
-            E T1 -> E T2 -> Prop)
-        (VR_E : forall T1 T2,
-            E T1 -> T1 -> E T2 -> T2 -> Prop).
+Lemma eq_globs : p_globs p1 = p_globs p2.
+Proof. done. Qed.
 
-
-
-
-(*Local Notation RS := (PR estate).
-Local Notation RV := (PR values).
-Local Notation RV1 := (PR value).
-Local Notation RSMV := (PR (syscall_state * mem * seq value)).
-*)
-
-Context (FI: FIso (void1 +' ErrEvent) E).
-
-(*
-Local Notation VS := (values * estate)%type.
-Local Notation FVS := (funname * VS)%type.
-
-Notation RVS := (fun (vs_st1 vs_st2 : VS) =>
-  (RV vs_st1.1 vs_st2.1 /\ RS vs_st1.2 vs_st2.2)).
-Notation RFVS := (fun (fvs1 fvs2 : FVS) =>
-  (fvs1.1 = fvs2.1 /\ RVS fvs1.2 fvs2.2)).
-Notation RC := (fun c1 c2: cmd => c2 = Tr_cmd c1).
-Notation RFunDef := (fun f1 f2: FunDef => f2 = Tr_FunDef f1).
-
-
-Context (rvs_def : PR VS = RVS)
-        (rfvs_def : PR FVS = RFVS)
-        (rc_def : PR cmd = RC)
-        (rfundef_def : PR FunDef = RFunDef).
-
-*)
-
-Context (HasErr: ErrEvent -< E).
-Context (wE: with_Error E).
-
-Definition RC c1 c2 := Tr_cmd c1 = c2.
-
-Context
-   (Rv  : value -> value -> Prop)
-   (Rscs: syscall_state_t -> syscall_state_t -> Prop)
-   (Rm  : mem -> mem -> Prop)
-   (RS  : estate -> estate -> Prop).
-
-Notation Rvs := (List.Forall2 Rv).
-
-Definition Rfres (fres1 fres2 : syscall_state_t * mem * values) :=
-   [/\ Rscs fres1.1.1 fres2.1.1
-      , Rm fres1.1.2 fres2.1.2
-      & Rvs fres1.2 fres2.2].
-
-Section TR_MutualRec.
-
-(* ME: relation between FCState events *)
-Definition TR_D_ME {T1 T2} (d1 : FCState T1)
-                           (d2 : FCState T2) : Prop :=
-  match d1, d2 with
-  | FLCode c1 st1, FLCode c2 st2 => RC c1 c2 /\ RS st1 st2
-  | FFCall scs1 m1 fn1 vs1, FFCall scs2 m2 fn2 vs2 =>
-    [/\ Rscs scs1 scs2
-      , Rm m1 m2
-      , fn1 = fn2
-      & Rvs vs1 vs2]
-  | _, _ => False
-  end.
-
-(* ME: relation between FCState event outputs, i.e. over estate *)
-Definition VR_D_ME {T1 T2}
-  (d1 : FCState T1) (t1: T1) (d2 : FCState T2) (t2: T2) : Prop :=
-  match d1 in FCState T1_ return T1_ -> T2 -> Prop with
-  | FLCode _ _ =>
-    match d2 in FCState T2_ return estate -> T2_ -> Prop with
-    | FLCode _ _ => RS
-    | FFCall _ _ _ _ => fun _ _ => False
-    end
-  | FFCall _ _ _ _ =>
-    match d2 in FCState T2_ return syscall_state_t * mem * values -> T2_ -> Prop with
-    | FLCode _ _ => fun _ _ => False
-    | FFCall _ _ _ _ => Rfres
-    end
-  end t1 t2.
-
-(***)
-
-Definition TR_DE : prerel (FCState +' E) (FCState +' E) :=
-  sum_prerel (@TR_D_ME) TR_E.
-
-Definition VR_DE : postrel (FCState +' E) (FCState +' E) :=
-  sum_postrel (@VR_D_ME) VR_E.
-
-(*
-Context (fcstate_t_def : TR_E (FCState +' E) = TR_DE_ME).
-Context (fcstate_v_def : VR_E (FCState +' E) = VR_DE_ME).
-*)
-(*
-Lemma rutt_err_eval_Args fn es1 st1 st2 :
-  RS st1 st2 ->
-  rutt (TR_E (FCState +' E)) (VR_E (FCState +' E)) RV
-    (err_eval_Args dc spp pr1 fn es1 st1)
-    (err_eval_Args dc spp pr2 fn (tr_exprs es1) st2).
-Admitted.
-
-Lemma rutt_err_init_state fn r1 r2 st1 st2 :
-  RV r1 r2 ->
-  RS st1 st2 ->
-  rutt (TR_E (FCState +' E)) (VR_E (FCState +' E)) RS
-    (err_init_state dc scP ev pr1 fn r1 st1)
-    (err_init_state dc scP ev pr2 fn r2 st2).
-Admitted.
-
-Lemma rutt_err_get_FunCode fn :
-  rutt (TR_E (FCState +' E)) (VR_E (FCState +' E)) RC
-    (err_get_FunCode pr1 fn)
-    (err_get_FunCode pr2 fn).
-Admitted.
-
-Lemma rutt_err_return_val fn st1 st2 :
-  RS st1 st2 ->
-  rutt (TR_E (FCState +' E)) (VR_E (FCState +' E)) RV
-    (err_return_val dc pr1 fn st1)
-    (err_return_val dc pr2 fn st2).
-Admitted.
-
-Lemma rutt_err_reinstate_caller fn xs v1 v2 st1 st2 st3 st4 :
-  RV v1 v2 ->
-  RS st1 st2 ->
-  RS st3 st4 ->
-  rutt (TR_E (FCState +' E)) (VR_E (FCState +' E))
-    RS
-    (err_reinstate_caller dc spp scP pr1 fn xs v1
-       st1 st3)
-    (err_reinstate_caller dc spp scP pr2 fn
-       (tr_lvals xs) v2 st2 st4).
-Admitted.
-*)
-(***)
-
-Check @rutt.
-(*
-(m_t : Type)
-(tr_e : m_t -> pexpr -> cexec pexpr)
-(tr_lval : m_t -> lval ->
-
- dead_code_i i O -> I, c
-
-s     -i-> s'
-={I}       ={O}
-t     -c-> t'
-
-
-s.mem = t.mem
-
-RS X s t : exists2 vm , t = with_vm s vm & s.(evm) <=[X] vm.
-RC I O cs ct = dead_code cs O = ok (I, ct).
-
-fres
-Definition Rfres (fres1 fres2 : syscall_state_t * mem * values) :=
-   [/\ Rscs fres1.1.1 fres2.1.1
-      , Rm fres1.1.2 fres2.1.2
-      & List.Forall2 values_uincl fres1.2 fres2.2].
-
-
-
-
-
-
-Let Pi_r s (i:instr_r) s' :=
-    forall ii s2,
-      match dead_code_i is_move_op do_nop onfun (MkI ii i) s2 with
-      | Ok (s1, c') =>
-        forall vm1', s.(evm) <=[s1] vm1' ->
-          exists vm2', s'.(evm) <=[s2] vm2' /\
-          sem_oi (with_vm s vm1') c' (with_vm s' vm2')
-      | _ => True
-      end.
-
-*)
-
-Lemma rutt_err_assgn x tg ty e st1 st2 :
-  RS st1 st2 ->
-  rutt_err TR_DE VR_DE RS
-    (iresult st1 (eval_assgn pr1 x tg ty e st1))
-    (iresult st2 (eval_assgn pr2 (tr_lval x) tg ty (tr_expr e) st2)).
+Lemma tr_exprsP wdb es :
+  requiv eq
+         ((sem_pexprs wdb (p_globs p1))^~ es)
+         ((sem_pexprs wdb (p_globs p2))^~ (tr_exprs es))
+         eq.
 Proof.
-  move=> hrs; apply rutt_iresult.
 Admitted.
 
-Lemma rutt_err_opn x o e st1 st2 :
-  RS st1 st2 ->
-  rutt_err TR_DE VR_DE RS
-    (iresult st1 (sem_sopn (p_globs pr1) o st1 x e))
-    (iresult st2 (sem_sopn (p_globs pr2) o st2 (tr_lvals x) (tr_exprs e))).
-Admitted.
-
-(*
-Lemma sum_postrelI (E1 E2 D1 D2 : Type -> Type) (PR1 : postrel E1 D1) (PR2 : postrel E2 D2) :
-  sum_postrel PR1 PR2
-: postrel (E1 +' E2) (D1 +' D2) :=
-    sum_postrel_inl : forall (A B : Type) (e1 : E1 A) (d1 : D1 B) (a : A) (b : B),
-                      PR1 A B e1 a d1 b -> sum_postrel PR1 PR2 A B (inl1 e1) a (inl1 d1) b
-  | sum_postrel_inr : forall (A B : Type) (e2 : E2 A) (d2 : D2 B) (a : A) (b : B),
-                      PR2 A B e2 a d2 b -> sum_postrel PR1 PR2 A B (inr1 e2) a (inr1 d2) b.
-*)
-Lemma rutt_msem_i (i: instr_r) (st1 st2: estate) :
-  RS st1 st2 ->
-  rutt_err TR_DE VR_DE RS (msem_i pr1 i st1) (msem_i pr2 (Tr_ir i) st2).
+Lemma tr_lvalsP wdb xs vs :
+  requiv eq (fun s0 : estate => write_lvals wdb (p_globs p1) s0 xs vs)
+    (fun s2 : estate => write_lvals wdb (p_globs p2) s2 (tr_lvals xs) vs) eq.
 Proof.
-  case: i.
-  + by move=> x tag ty e hst /=; apply rutt_err_assgn.
-  + admit.
-  + admit.
-  + move=> e c1 c2 hst.
-(*
-    Opaque msem_i.
-rewrite /=.
-
-RC_bw I O c1 c2 =  dead_code_c c1 O = ok (I, c2)
-RC_fw I O c1 c2 =  const_prop_c c1 I = ok (O, c2)
-
-TR_D_ME I O =
-fun (T1 T2 : Type) (d1 : FCState T1) (d2 : FCState T2) =>
-match d1 with
-| FLCode c1 st1 => match d2 with
-                   | FLCode c2 st2 => RC I O c1 c2 /\ RS I st1 st2
-                   | FFCall _ _ _ _ => False
-                   end
-| FFCall scs1 m1 fn1 vs1 =>
-    match d2 with
-    | FLCode _ _ => False
-    | FFCall scs2 m2 fn2 vs2 => [/\ Rscs scs1 scs2, Rm m1 m2, fn1 = fn2 & Rvs vs1 vs2]
-    end
-end
-
-VR_D_ME I O =
-fun (T1 T2 : Type) (d1 : FCState T1) (d2 : FCState T2) =>
-match d1 with
-| FLCode c1 st1 => match d2 with
-                   | FLCode c2 st2 => RS O st1 st2
-                   | FFCall _ _ _ _ => False
-                   end
-| FFCall scs1 m1 fn1 vs1 =>
-    match d2 with
-    | FLCode _ _ => False
-    | FFCall scs2 m2 fn2 vs2 => [/\ Rscs scs1 scs2, Rm m1 m2, fn1 = fn2 & Rvs vs1 vs2]
-    end
-end
-
-[/\ Rscs scs1 scs2, Rm m1 m2, fn1 = fn2 & Rvs vs1 vs2]
-Rscs Rm Rvs = eq
-Rscs Rm = eq, Rvs = List.Forall2 value_uincl.
-
-
-
-
-
-
-forall O,
-
- rutt_err TR_DE VR_DE RS (msem_i pr1 (Cif e c1 c2) st1) (msem_i pr2 (Cif e' c1' c2') st2).
-
-
- /=.
-*)
-    apply rutt_bind with (RR := eq).
-    + admit.
-    move=> b _ <-.
-    apply rutt_trigger => /=.
-    + by apply sum_prerel_inl => /=; split => //; case: b.
-    by move=> t1 t2 h; dependent destruction h; auto.
-  + admit.
-  + move=> al c1 e c2 hst /=.
-    apply XRuttFacts.rutt_iter with (RI:=RS) => //.
-    move=> s1 s2 hs.
-    apply rutt_bind with (RR := RS).
-    + apply rutt_trigger => /=.
-      + by apply sum_prerel_inl => /=.
-      by move=> t1 t2 h; dependent destruction h; auto.
-    move=> t1 t2 ht.
-    apply rutt_bind with (RR := eq).
-    + admit.
-    move=> b _ <-.
-    case: b.
-    + apply rutt_bind with (RR := RS).
-      + apply rutt_trigger => /=.
-        + by apply sum_prerel_inl.
-        by move=> ?? h; dependent destruction h; auto.
-      by move=> ?? h; apply rutt_Ret; constructor.
-    by apply rutt_Ret; constructor.
-  move=> xs fn es hst /=.
-  apply rutt_bind with (RR := Rvs).
-  + admit.
-  move=> vs1 vs2 hvs.
-  apply rutt_bind with (RR := Rfres).
-  + apply rutt_trigger => /=.
-    + apply sum_prerel_inl => /=; split => //.
-      + admit. (* RS => Rscs *)
-      admit. (* RS => Rmem *)
-    move=> ?? h; dependent destruction h; auto.
-  move=> [[scs2 m2] vs] [[scs2' m2'] vs'] [/=???].
-  admit.
 Admitted.
 
-Lemma rutt_msem_fcstate ev1 ev2 T1 T2 (d1 : FCState T1) (d2: FCState T2) :
-  TR_D_ME d1 d2 ->
-  rutt_err TR_DE VR_DE (fun v1 v2 => VR_D_ME d1 v1 d2 v2) (msem_fcstate pr1 ev1 d1) (msem_fcstate pr2 ev2 d2).
-Proof.
-  case: d1 d2 => [c1 st1 | scs1 m1 f1 vs1]  [c2 st2 | scs2 m2 f2 vs2] //=.
-  + move=> [<- hst].
-    elim: c1 st1 st2 hst => [ | [ii i] c hrec] st1 st2 hst /=.
-    + by apply rutt_Ret.
-    apply rutt_bind with (RR := RS) => //.
-    by apply rutt_msem_i.
-  move=> [hscs hm <- hvs].
-  rewrite /msem_call.
-  apply rutt_bind with (RR := fun fd1 fd2 => fd2 = Tr_FunDef fd1).
-  + admit.
+Lemma tr_cond e :
+ requiv eq (sem_cond (p_globs p1) e) (sem_cond (p_globs p2) (tr_expr e)) eq.
 Admitted.
 
-Lemma rutt_rsem_call ev1 ev2 scs1 m1 fn vs1 scs2 m2 vs2 :
-  Rfres (scs1, m1, vs1)  (scs2, m2, vs2) ->
-  rutt_err TR_E VR_E Rfres (rsem_call pr1 ev1 scs1 m1 fn vs1) (rsem_call pr2 ev2 scs2 m2 fn vs2).
+Lemma tr_bound lo hi :
+ requiv eq (sem_bound (p_globs p1) lo hi) (sem_bound (p_globs p2) (tr_expr lo) (tr_expr hi)) eq.
+Admitted.
+
+Lemma Tr_fundefP fn : equiv_f p1 p2 ev ev RPreFeq fn fn RPostFeq.
 Proof.
-  move=> hpre; apply interp_mrec_rutt_err with (RPreInv := @TR_D_ME) (RPostInv := @VR_D_ME).
-  + move=> T1 T2 d1 d2.
-    by apply rutt_msem_fcstate.
-  have := @rutt_msem_fcstate ev1 ev2 _ _ (FFCall scs1 m1 fn vs1) (FFCall scs2 m2 fn vs2).
-  apply => /=; case hpre => //.
+ apply isem_fun_ind => hrec {fn}.
+ move=> fn _ fs _ [<- <-] fd hget.
+ exists (tr_fundef fd).
+ + by rewrite get_map_prog hget.
+ move=> {hget}; exists eq, eq => s1 hinit.
+ exists s1; split => //; last first.
+ + by move=> s1' _ fr1 <- hfinal; exists fr1.
+ set Pi := fun (i:instr) => equiv_rec p1 p2 ev ev RPreFeq RPostFeq eq [::i] [::tr_i i] eq.
+ set Pr := fun (i:instr_r) => forall ii, Pi (MkI ii i).
+ set Pc := fun (c:cmd) => equiv_rec p1 p2 ev ev RPreFeq RPostFeq eq c (tr_c c) eq.
+ move=> {fn fs hinit}.
+ apply (cmd_rect (Pr := Pr) (Pi:=Pi) (Pc:=Pc)) => // {fd}.
+ + by apply equiv_nil.
+ + by move=> i c; apply equiv_cons.
+ + move=> x tg ty e ii; apply equiv_assgn with eq eq.
+   + by rewrite -eq_globs; apply tr_exprP.
+   + by move=> v _ v' <-; eauto.
+   by move=> v _ <-; rewrite -eq_globs; apply tr_lvalP.
+ + move=> xs t o es ii; apply equiv_opn with eq eq.
+   + by apply tr_exprsP.
+   + by move=> vs _ vs' <-; eauto.
+   by move=> vs _ <-; apply tr_lvalsP.
+ + move=> xs o es ii; apply equiv_syscall with eq eq.
+   + by apply tr_exprsP.
+   + by move=> vs _ <- s _ fs <-; eauto.
+   move=> scs m vs _ _ _ [<- <- <-].
+   by move=> s _ s' <-; apply tr_lvalsP.
+ + move=> e c1 c2 hc1 hc2 ii; apply equiv_if => //.
+   by apply tr_cond.
+ + move=> j d lo hi c hc ii; apply equiv_for with eq => //.
+   + by apply tr_bound.
+   by move=> i s _ s' <-; eauto.
+ + move=> al c e c' hc hc' ii; apply equiv_while => //.
+   by apply tr_cond.
+ move=> xs f es ii; apply equiv_call with RPreFeq RPostFeq eq.
+ + by apply tr_exprsP.
+ + by move=> s _ vs _ <- <-.
+ + by apply hrec.
+ move=> fs1 fs2 fr _ _ <-.
+ by move=> s _ s' <-; apply tr_lvalsP.
 Qed.
 
-
-(*
-
-Search interp_err.
-
-Definition rsem_call {E} `{ErrEvent -< E}
-   (scs1 : syscall_state_t) (m1 : mem)
-   (fn : funname) (vargs : values) : itree E (syscall_state_t * mem * values) :=
- mrec msem_fcstate (FFCall scs1 m1 fn vargs).
-
-
-
-Lemma rutt_err_mk_SyscallE x sc e st1 st2 :
-  RS st1 st2 ->
-  rutt (sum_prerel (@TR_D_ME) (TR_E E)) (sum_postrel (@VR_D_ME) (VR_E E)) RS
-    (err_mk_SyscallE spp scP pr1 x sc e st1)
-    (err_mk_SyscallE spp scP pr2
-       (tr_lvals x) (tr_sysc sc) (tr_exprs e) st2).
-Admitted.
-
-Lemma rutt_err_mk_EvalCond e st1 st2 :
-  RS st1 st2 ->
-   rutt (sum_prerel (@TR_D_ME) (TR_E E)) (sum_postrel (@VR_D_ME) (VR_E E)) eq
-    (err_mk_EvalCond spp pr1 e st1)
-    (err_mk_EvalCond spp pr2 (tr_expr e) st2).
-Admitted.
-
-Lemma rutt_err_mk_EvalBound e st1 st2 :
-  RS st1 st2 ->
-  rutt (sum_prerel (@TR_D_ME) (TR_E E)) (sum_postrel (@VR_D_ME) (VR_E E)) eq
-    (err_mk_EvalBound spp pr1 e st1)
-    (err_mk_EvalBound spp pr2 e st2).
-Admitted.
-
-Lemma rutt_err_mk_WriteIndex xi z st1 st2 :
-  RS st1 st2 ->
-   rutt (sum_prerel (@TR_D_ME) (TR_E E)) (sum_postrel (@VR_D_ME) (VR_E E)) RS
-    (err_mk_WriteIndex xi z st1) (err_mk_WriteIndex xi z st2).
-Admitted.
-*)
-(*
-Lemma comp_gen_ok_ME (fn: funname)
-  (xs1 xs2: lvals) (es1 es2: pexprs) (st1 st2: estate) :
-  xs2 = map tr_lval xs1 ->
-  es2 = map tr_expr es1 ->
-  RS st1 st2 ->
-  rutt_err TR_DE VR_DE
-   (msem_i
-
-
- (FCState +' E) _ _ _ (TR_E _) (VR_E _)
-    (fun a1 a2 => @VR_D_ME _ _ (FFCall_ xs1 fn es1 st1) a1
-                             (FFCall_ xs2 fn es2 st2) a2)
-    (meval_fcall pr1 xs1 fn es1 st1) (meval_fcall pr2 xs2 fn es2 st2).
-  intros.
-  unfold meval_fcall; simpl.
-
-  eapply rutt_bind with (RR := RV); inv H; intros.
-
-  { eapply rutt_err_eval_Args; auto. }
-
-  eapply rutt_bind with (RR := RS); intros.
-
-  { eapply rutt_err_init_state; auto. }
-
-  eapply rutt_bind with (RR := RC); intros.
-
-  { eapply rutt_err_get_FunCode; auto. }
-
-  inv H2. eapply rutt_bind with (RR := RS); intros.
-  { eapply rutt_trigger; simpl; intros.
-    { rewrite fcstate_t_def.
-      econstructor.
-      split; auto; intros.
-    }
-    rewrite fcstate_v_def in H2.
-    dependent destruction H2.
-    unfold VR_D_ME in H2; auto.
-  }
-
-  eapply rutt_bind with (RR := RV); intros.
-  { eapply rutt_err_return_val; auto. }
-
-  assert ((fun a1 : estate => [eta RS a1]) = RS) as A1.
-  { eauto. }
-
-  rewrite A1; eapply rutt_err_reinstate_caller; auto.
-Qed.
-*)
-(* Inductive lemma - GOOD. here we are not tying the coinductive knot,
-   as st_cmd_map_r is just a map function. *)
-(*
-Lemma rutt_cmd_tr_ME_step (cc: cmd) (st1 st2: estate) :
-  RS st1 st2 ->
-  rutt_err (FCState +' E) _ _ _
-    (sum_prerel (@TR_D_ME) (TR_E E))
-    (sum_postrel (@VR_D_ME) (VR_E E))
-    RS (st_cmd_map_r (meval_instr pr1) cc st1)
-    (st_cmd_map_r (meval_instr pr2) (Tr_cmd cc) st2).
-  simpl; intros.
-
-  set (Pr := fun (i: instr_r) => forall ii st1 st2, RS st1 st2 ->
-     @rutt (FCState +' E) _ _ _
-    (sum_prerel (@TR_D_ME) (TR_E E))
-    (sum_postrel (@VR_D_ME) (VR_E E))
-    RS
-    (st_cmd_map_r (meval_instr pr1) ((MkI ii i) :: nil) st1)
-    (st_cmd_map_r (meval_instr pr2) ((Tr_instr (MkI ii i)) :: nil) st2)).
-
-  set (Pi := fun (i: instr) => forall st1 st2, RS st1 st2 ->
-     @rutt (FCState +' E) _ _ _
-    (sum_prerel (@TR_D_ME) (TR_E E))
-    (sum_postrel (@VR_D_ME) (VR_E E))
-    RS
-    (st_cmd_map_r (meval_instr pr1) (i :: nil) st1)
-    (st_cmd_map_r (meval_instr pr2) ((Tr_instr i) :: nil) st2)).
-
-  set (Pc := fun (c: cmd) => forall st1 st2, RS st1 st2 ->
-     @rutt (FCState +' E) _ _ _
-    (sum_prerel (@TR_D_ME) (TR_E E))
-    (sum_postrel (@VR_D_ME) (VR_E E))
-    RS
-    (st_cmd_map_r (meval_instr pr1) c st1)
-    (st_cmd_map_r (meval_instr pr2) (Tr_cmd c) st2)).
-
-  revert H; revert st1 st2; revert cc.
-  apply (cmd_Ind Pr Pi Pc); rewrite /Pr /Pi /Pc; simpl; eauto; intros.
-
-  { eapply rutt_Ret; eauto. }
-  { destruct i; simpl.
-    eapply rutt_bind with (RR := RS); simpl in *.
-
-    specialize (H st1 st2 H1).
-
-    setoid_rewrite bind_ret_r in H; auto.
-    intros; auto.
-  }
-
-  { eapply rutt_bind with (RR := RS); intros.
-    eapply rutt_err_mk_AssgnE; auto.
-    eapply rutt_Ret; eauto.
-  }
-
-  { eapply rutt_bind with (RR := RS); intros.
-    eapply rutt_err_mk_OpnE; auto.
-    eapply rutt_Ret; eauto.
-  }
-
-  { eapply rutt_bind with (RR := RS); intros.
-    eapply rutt_err_mk_SyscallE; auto.
-    eapply rutt_Ret; eauto.
-  }
-
-  { intros.
-    eapply rutt_bind with (RR := RS); intros.
-    { eapply rutt_bind with (RR := eq); intros.
-      { eapply rutt_err_mk_EvalCond; auto. }
-      inv H2; destruct r2; simpl.
-      eapply H; eauto.
-      eapply H0; eauto.
-    }
-    eapply rutt_Ret; auto.
-  }
-
-  { eapply rutt_bind with (RR := RS); simpl; intros.
-    destruct rn; destruct p; simpl.
-    eapply rutt_bind with (RR := eq); simpl; intros.
-    eapply rutt_err_mk_EvalBound; auto.
-
-    inv H1; eapply rutt_bind with (RR := eq); simpl; intros.
-    eapply rutt_err_mk_EvalBound; auto.
-
-    inv H1; revert H0; revert st1 st2.
-    induction (wrange d r2 r0); simpl; intros.
-    { eapply rutt_Ret; eauto. }
-    { eapply rutt_bind with (RR:= RS); simpl; intros.
-      { eapply rutt_err_mk_WriteIndex; auto. }
-      eapply rutt_bind with (RR := RS); intros; auto.
-    }
-
-    eapply rutt_Ret; auto.
-  }
-
-  { eapply rutt_bind with (RR := RS); intros.
-    eapply rutt_iter with (RI := RS); intros; auto.
-    eapply rutt_bind with (RR := RS); intros.
-    eapply H; auto.
-
-    eapply rutt_bind with (RR := eq); intros.
-    eapply rutt_err_mk_EvalCond; auto.
-
-    inv H4; destruct r3.
-
-    eapply rutt_bind with (RR := RS); intros; auto.
-    eapply rutt_Ret; auto.
-    eapply rutt_Ret; auto.
-    eapply rutt_Ret; auto.
-  }
-
-  { eapply rutt_bind with (RR := RS); intros.
-    eapply rutt_trigger; simpl; intros.
-    econstructor.
-    unfold TR_D_ME; simpl.
-    split; eauto.
-
-    simpl in H0.
-
-    intros; auto.
-    simpl in H0.
-    dependent destruction H0; auto.
-    eapply rutt_Ret; auto.
-  }
-Qed.
-
-(* Here we apply the inductive lemma and comp_gen_ok *)
-Lemma rutt_cmd_tr_ME (cc: cmd) (st1 st2: estate) :
-  RS st1 st2 ->
-  @rutt E _ _ _
-    (TR_E _) (VR_E _) RS
-    (mevalE_cmd pr1 cc st1) (mevalE_cmd pr2 (Tr_cmd cc) st2).
-Proof.
-  intros; unfold mevalE_cmd; simpl.
-  eapply interp_mrec_rutt; simpl; intros.
-  { instantiate (3 := @TR_D_ME).
-    instantiate (1 := @VR_D_ME).
-    unfold meval_cstate.
-    destruct d1.
-    { unfold TR_D_ME in H0.
-      destruct d2; try intuition.
-      inv H1; simpl.
-      eapply rutt_cmd_tr_ME_step; eauto.
-    }
-
-    { unfold TR_D_ME in H0.
-      destruct d2; simpl in *; try intuition.
-      inv H0.
-      have CC := (comp_gen_ok_ME f0 xs _ es _ _ _ erefl erefl H4).
-      setoid_rewrite fcstate_t_def in CC.
-      setoid_rewrite fcstate_v_def in CC.
-      eapply CC.
-    }
-  }
-  eapply rutt_cmd_tr_ME_step; eauto.
-Qed.
-*)
-
-End TR_MutualRec.
-
-End TR_tests.
-
-End TRANSF.
-
-End WSW.
+End TEST.
 
 
 
